Working on connecting high-level Merkle tree design and spec

secure_api/merkle_tree/MerkleTree.New.High.fst
@@ -5,7 +5,7 @@ open EverCrypt.Helpers
 
 open MerkleTree.Spec
 
-open FStar.All
+open FStar.Classical
 open FStar.Ghost
 open FStar.Seq
 
@@ -49,33 +49,64 @@ val mt_not_full: merkle_tree -> GTot bool
 let mt_not_full mt =
   MT?.j mt < pow2 merkle_tree_size_lg - 1
 
-/// Well-formedness
+val mt_empty: merkle_tree -> GTot bool
+let mt_empty mt =
+  MT?.j mt = 0
+
+val mt_not_empty: merkle_tree -> GTot bool
+let mt_not_empty mt =
+  MT?.j mt > 0
+
+val log_of: n:nat{n > 0} -> GTot nat
+let rec log_of n =
+  if n = 1 then 0
+  else 1 + log_of (n / 2)
+
+val log_of_bound:
+  m:nat -> n:nat{n > 0 && n < pow2 m} ->
+  Lemma (log_of n < m)
+        [SMTPatOr [[SMTPat (n < pow2 m)]; [SMTPat (n < pow2 m - 1)]]]
+let rec log_of_bound m n =
+  if n = 1 then ()
+  else log_of_bound (m - 1) (n / 2)
+
+val mt_depth: mt:merkle_tree{mt_not_empty mt} -> GTot nat
+let mt_depth mt = log_of (MT?.j mt)
+
+val mt_depth_ok:
+  mt:merkle_tree{mt_not_empty mt} ->
+  Lemma (S.length (MT?.hs mt) > mt_depth mt)
+        [SMTPat (mt_depth mt)]
+let mt_depth_ok mt =
+  log_of_bound merkle_tree_size_lg (MT?.j mt)
+
+/// Well-formedness w.r.t. indices of base hash elements
 
 val offset_of: i:nat -> Tot nat
 let offset_of i =
   if i % 2 = 0 then i else i - 1
 
-val mt_wf_elts:
+val hs_wf_elts:
   lv:nat{lv <= 32} ->
   hs:hash_ss{S.length hs = 32} ->
   i:nat -> j:nat{j >= i} ->
   GTot Type0 (decreases (32 - lv))
-let rec mt_wf_elts lv hs i j =
+let rec hs_wf_elts lv hs i j =
   if lv = 32 then true
   else (let ofs = offset_of i in
        S.length (S.index hs lv) == j - ofs /\
-       mt_wf_elts (lv + 1) hs (i / 2) (j / 2))
+       hs_wf_elts (lv + 1) hs (i / 2) (j / 2))
 
-val mt_wf_elts_equal:
+val hs_wf_elts_equal:
   lv:nat{lv <= 32} ->
   hs1:hash_ss{S.length hs1 = 32} ->
   hs2:hash_ss{S.length hs2 = 32} ->
   i:nat -> j:nat{j >= i} ->
-  Lemma (requires (mt_wf_elts lv hs1 i j /\
+  Lemma (requires (hs_wf_elts lv hs1 i j /\
 		  S.equal (S.slice hs1 lv 32) (S.slice hs2 lv 32)))
-	(ensures (mt_wf_elts lv hs2 i j))
+	(ensures (hs_wf_elts lv hs2 i j))
 	(decreases (32 - lv))
-let rec mt_wf_elts_equal lv hs1 hs2 i j =
+let rec hs_wf_elts_equal lv hs1 hs2 i j =
   if lv = 32 then ()
   else (S.slice_slice hs1 lv 32 1 (32 - lv);
        S.slice_slice hs2 lv 32 1 (32 - lv);
@@ -84,30 +115,101 @@ let rec mt_wf_elts_equal lv hs1 hs2 i j =
        S.lemma_index_slice hs1 lv 32 0; 
        S.lemma_index_slice hs2 lv 32 0;
        assert (S.index hs1 lv == S.index hs2 lv);
-       mt_wf_elts_equal (lv + 1) hs1 hs2 (i / 2) (j / 2))
+       hs_wf_elts_equal (lv + 1) hs1 hs2 (i / 2) (j / 2))
 
-val mt_wf: merkle_tree -> GTot Type0
-let mt_wf mt =
-  mt_wf_elts 0 (MT?.hs mt) (MT?.i mt) (MT?.j mt)
+val mt_wf_elts: merkle_tree -> GTot Type0
+let mt_wf_elts mt =
+  hs_wf_elts 0 (MT?.hs mt) (MT?.i mt) (MT?.j mt)
 
-type wf_mt = mt:merkle_tree{mt_wf mt}
+/// Connection to Merkle tree specification
+
+val merge_hs: 
+  hs1:hash_ss -> hs2:hash_ss{S.length hs1 = S.length hs2} -> 
+  GTot (mhs:hash_ss{S.length mhs = S.length hs1})
+       (decreases (S.length hs1))
+let rec merge_hs hs1 hs2 =
+  if S.length hs1 = 0 then S.empty
+  else S.cons (S.append (S.head hs1) (S.head hs2))
+              (merge_hs (S.tail hs1) (S.tail hs2))
+
+val hash_ss_length_in_spec: 
+  n:nat -> fhs:hash_ss -> GTot Type0
+let rec hash_ss_length_in_spec n fhs =
+  S.length fhs = n + 1 /\
+  (forall (i:nat{i <= n}). S.length (S.index fhs i) <= pow2 (n - i))
+
+val hash_seq_lift: hs:hash_seq -> GTot MTS.hash_seq (decreases (S.length hs))
+let rec hash_seq_lift hs =
+  if S.length hs = 0 then S.empty
+  else S.cons (HRaw (S.head hs)) (hash_seq_lift (S.tail hs))
+
+val hash_seq_in_spec:
+  n:nat -> hs:hash_seq{S.length hs <= pow2 n} -> smt:MTS.merkle_tree n -> GTot Type0
+let hash_seq_in_spec n hs smt =
+  S.equal (hash_seq_lift hs) (S.slice smt 0 (S.length hs))
+
+// `fhs` should contain deprecated hashes.
+val hash_ss_in_spec:
+  #n:nat -> fhs:hash_ss{hash_ss_length_in_spec n fhs} ->
+  smt:MTS.merkle_tree n ->
+  GTot Type0
+let rec hash_ss_in_spec #n fhs smt =
+  if n = 0 then hash_seq_in_spec n (S.head fhs) smt
+  else hash_ss_in_spec #(n-1) (S.tail fhs) (mt_next_lv smt)
+
+// NOTE: unlike actual high-level design, here `rhs` should contain the root!
+val hs_wf_rpmt_:
+  #n:nat ->
+  olds:hash_ss{S.length olds = n + 1} ->
+  hs:hash_ss{S.length hs = n + 1} ->
+  smt:MTS.merkle_tree n ->
+  GTot Type0
+let hs_wf_rpmt_ #n olds hs smt =
+  hash_ss_length_in_spec n (merge_hs olds hs) /\
+  hash_ss_in_spec #n (merge_hs olds hs) smt
+
+val hs_wf_rpmt: n:nat -> hs:hash_ss{S.length hs = n + 1} -> GTot Type0
+let hs_wf_rpmt n hs =
+  exists (olds:hash_ss{S.length olds = n + 1}) 
+         (smt:MTS.merkle_tree n).
+    hs_wf_rpmt_ #n olds hs smt
+
+val hs_wf_rpmt_ex:
+  n:nat -> hs:hash_ss{S.length hs = n + 1} ->
+  olds:hash_ss{S.length olds = n + 1} -> 
+  smt:MTS.merkle_tree n ->
+  Lemma (requires (hs_wf_rpmt_ #n olds hs smt))
+        (ensures (hs_wf_rpmt n hs))
+let hs_wf_rpmt_ex n hs olds smt =
+  exists_intro (fun smt -> hs_wf_rpmt_ #n olds hs smt) smt;
+  exists_intro
+    (fun (olds:hash_ss{S.length olds = n + 1}) ->
+      exists smt. hs_wf_rpmt_ #n olds hs smt) olds
+
+val mt_wf_rpmt: mt:merkle_tree -> GTot Type0
+let mt_wf_rpmt mt =
+  mt_empty mt \/
+  // See [SMTPat] in `mt_depth_ok` to check why below `S.slice` works.
+  hs_wf_rpmt (mt_depth mt) (S.slice (MT?.hs mt) 0 (mt_depth mt + 1))
 
 /// Construction
 
-val mt_wf_elts_empty:
+val hs_wf_elts_empty:
   lv:nat{lv <= 32} ->
   Lemma (requires True)
-	(ensures (mt_wf_elts lv (S.create 32 S.empty) 0 0))
+	(ensures (hs_wf_elts lv (S.create 32 S.empty) 0 0))
 	(decreases (32 - lv))
-let rec mt_wf_elts_empty lv =
+let rec hs_wf_elts_empty lv =
   if lv = 32 then ()
-  else mt_wf_elts_empty (lv + 1)
+  else hs_wf_elts_empty (lv + 1)
 
 // NOTE: the public function is `create_mt` defined below, which
 // builds a tree with an initial hash.
-val create_empty_mt: unit -> GTot wf_mt
+// NOTE: the empty Merkle tree does not satisfy `mt_wf_rpmt` since it requires
+
+val create_empty_mt: unit -> GTot (mt:merkle_tree{mt_wf_elts mt /\ mt_wf_rpmt mt})
 let create_empty_mt _ =
-  mt_wf_elts_empty 0;
+  hs_wf_elts_empty 0;
   MT 0 0 (S.create 32 S.empty) false (S.create 32 hash_init) hash_init
 
 /// Insertion
@@ -116,19 +218,19 @@ val hash_ss_insert:
   lv:nat{lv < 32} ->
   i:nat ->
   j:nat{i <= j /\ j < pow2 (32 - lv) - 1} ->
-  hs:hash_ss{S.length hs = 32 /\ mt_wf_elts lv hs i j} ->
+  hs:hash_ss{S.length hs = 32 /\ hs_wf_elts lv hs i j} ->
   v:hash ->
-  GTot (ihs:hash_ss{S.length ihs = 32 /\ mt_wf_elts (lv + 1) ihs (i / 2) (j / 2)})
+  GTot (ihs:hash_ss{S.length ihs = 32 /\ hs_wf_elts (lv + 1) ihs (i / 2) (j / 2)})
 let hash_ss_insert lv i j hs v =
   let ihs = S.upd hs lv (S.snoc (S.index hs lv) v) in
-  mt_wf_elts_equal (lv + 1) hs ihs (i / 2) (j / 2);
+  hs_wf_elts_equal (lv + 1) hs ihs (i / 2) (j / 2);
   ihs
 
 val insert_:
   lv:nat{lv < 32} ->
   i:nat ->
   j:nat{i <= j /\ j < pow2 (32 - lv) - 1} ->
-  hs:hash_ss{S.length hs = 32 /\ mt_wf_elts lv hs i j} ->
+  hs:hash_ss{S.length hs = 32 /\ hs_wf_elts lv hs i j} ->
   acc:hash ->
   GTot (ihs:hash_ss{S.length ihs = 32})
        (decreases j)
@@ -143,7 +245,7 @@ val insert_base:
   lv:nat -> i:nat -> j:nat -> hs:hash_ss -> acc:hash ->
   Lemma (requires (
 	  lv < 32 /\ i <= j /\ j < pow2 (32 - lv) - 1 /\
-	  S.length hs = 32 /\ mt_wf_elts lv hs i j /\
+	  S.length hs = 32 /\ hs_wf_elts lv hs i j /\
 	  j % 2 <> 1))
 	(ensures (S.equal (insert_ lv i j hs acc)
 			  (hash_ss_insert lv i j hs acc)))
@@ -153,10 +255,10 @@ val insert_rec:
   lv:nat -> i:nat -> j:nat -> hs:hash_ss -> acc:hash ->
   Lemma (requires (
 	  lv < 32 /\ i <= j /\ j < pow2 (32 - lv) - 1 /\
-	  S.length hs = 32 /\ mt_wf_elts lv hs i j /\
+	  S.length hs = 32 /\ hs_wf_elts lv hs i j /\
 	  j % 2 == 1))
 	(ensures (
-	  (mt_wf_elts_equal (lv + 1) hs
+	  (hs_wf_elts_equal (lv + 1) hs
 	    (hash_ss_insert lv i j hs acc) (i / 2) (j / 2);
 	  S.equal (insert_ lv i j hs acc)
 		  (insert_ (lv + 1) (i / 2) (j / 2)
@@ -165,7 +267,7 @@ val insert_rec:
 let insert_rec lv i j hs acc = ()
 
 val mt_insert:
-  mt:wf_mt{mt_not_full mt} -> v:hash -> GTot merkle_tree
+  mt:merkle_tree{mt_wf_elts mt /\ mt_not_full mt} -> v:hash -> GTot merkle_tree
 let mt_insert mt v =
   MT (MT?.i mt)
      (MT?.j mt + 1)
@@ -192,7 +294,7 @@ val construct_rhs:
   i:nat ->
   j:nat{
     i <= j /\ j < pow2 (32 - lv) /\
-    mt_wf_elts lv hs i j} ->
+    hs_wf_elts lv hs i j} ->
   acc:hash ->
   actd:bool ->
   GTot (crhs:hash_seq{S.length crhs = 32} * hash) (decreases j)
@@ -215,7 +317,7 @@ val construct_rhs_even:
   i:nat ->
   j:nat{
     i <= j /\ j < pow2 (32 - lv) /\
-    mt_wf_elts lv hs i j} ->
+    hs_wf_elts lv hs i j} ->
   acc:hash ->
   actd:bool ->
   Lemma (requires (j <> 0 /\ j % 2 = 0))
@@ -230,7 +332,7 @@ val construct_rhs_odd:
   i:nat ->
   j:nat{
     i <= j /\ j < pow2 (32 - lv) /\
-    mt_wf_elts lv hs i j} ->
+    hs_wf_elts lv hs i j} ->
   acc:hash ->
   actd:bool ->
   Lemma (requires (j % 2 = 1))
@@ -244,7 +346,7 @@ val construct_rhs_odd:
 let construct_rhs_odd lv hs rhs i j acc actd = ()
 
 val mt_get_root: 
-  mt:wf_mt -> drt:hash ->
+  mt:merkle_tree{mt_wf_elts mt} -> drt:hash ->
   GTot (merkle_tree * hash)
 let mt_get_root mt drt =
   if MT?.rhs_ok mt then (mt, MT?.mroot mt)
@@ -257,13 +359,13 @@ let mt_get_root mt drt =
   end
 
 val mt_get_root_rhs_ok_true:
-  mt:wf_mt -> drt:hash ->
+  mt:merkle_tree{mt_wf_elts mt} -> drt:hash ->
   Lemma (requires (MT?.rhs_ok mt == true))
         (ensures (mt_get_root mt drt == (mt, MT?.mroot mt)))
 let mt_get_root_rhs_ok_true mt drt = ()
 
 val mt_get_root_rhs_ok_false:
-  mt:wf_mt -> drt:hash ->
+  mt:merkle_tree{mt_wf_elts mt} -> drt:hash ->
   Lemma (requires (MT?.rhs_ok mt == false))
         (ensures (mt_get_root mt drt ==
                  (let (nrhs, rt) = 
@@ -299,7 +401,7 @@ val mt_get_path_step:
   i:nat ->
   j:nat{
     j <> 0 /\ i <= j /\ j < pow2 (32 - lv) /\
-    mt_wf_elts lv hs i j} ->
+    hs_wf_elts lv hs i j} ->
   k:nat{i <= k && k <= j} ->
   p:path ->
   actd:bool ->
@@ -324,7 +426,7 @@ val mt_get_path_:
   i:nat -> 
   j:nat{
     i <= j /\ j < pow2 (32 - lv) /\
-    mt_wf_elts lv hs i j} ->
+    hs_wf_elts lv hs i j} ->
   k:nat{i <= k && k <= j} ->
   p:path ->
   actd:bool ->
@@ -339,7 +441,7 @@ let rec mt_get_path_ lv hs rhs i j k p actd =
     		 (if j % 2 = 0 then actd else true))
 
 val mt_get_path: 
-  mt:wf_mt ->
+  mt:merkle_tree{mt_wf_elts mt} ->
   idx:nat{MT?.i mt <= idx /\ idx < MT?.j mt} ->
   drt:hash ->
   GTot (nat * 
@@ -361,7 +463,7 @@ val mt_flush_to_:
   i:nat{i >= pi} ->
   j:nat{
     j >= i /\ j < pow2 (32 - lv) /\
-    mt_wf_elts lv hs pi j} ->
+    hs_wf_elts lv hs pi j} ->
   GTot (fhs:hash_ss{S.length fhs = 32}) (decreases i)
 let rec mt_flush_to_ lv hs pi i j =
   let oi = offset_of i in
@@ -371,7 +473,7 @@ let rec mt_flush_to_ lv hs pi i j =
        let hvec = S.index hs lv in
        let flushed = S.slice hvec ofs (S.length hvec) in
        let nhs = S.upd hs lv flushed in
-       mt_wf_elts_equal (lv + 1) hs nhs (pi / 2) (j / 2);
+       hs_wf_elts_equal (lv + 1) hs nhs (pi / 2) (j / 2);
        mt_flush_to_ (lv + 1) nhs (pi / 2) (i / 2) (j / 2))
 
 val mt_flush_to_rec:
@@ -381,26 +483,26 @@ val mt_flush_to_rec:
   i:nat{i >= pi} ->
   j:nat{
     j >= i /\ j < pow2 (32 - lv) /\
-    mt_wf_elts lv hs pi j} ->
+    hs_wf_elts lv hs pi j} ->
   Lemma (requires (offset_of i <> offset_of pi))
         (ensures (mt_flush_to_ lv hs pi i j ==
                  (let ofs = offset_of i - offset_of pi in
                  let hvec = S.index hs lv in
                  let flushed = S.slice hvec ofs (S.length hvec) in
                  let nhs = S.upd hs lv flushed in
-                 mt_wf_elts_equal (lv + 1) hs nhs (pi / 2) (j / 2);
+                 hs_wf_elts_equal (lv + 1) hs nhs (pi / 2) (j / 2);
                  mt_flush_to_ (lv + 1) nhs (pi / 2) (i / 2) (j / 2))))
 let mt_flush_to_rec lv hs pi i j = ()                 
 
 val mt_flush_to: 
-  mt:wf_mt -> 
+  mt:merkle_tree{mt_wf_elts mt} -> 
   idx:nat{idx >= MT?.i mt /\ idx < MT?.j mt} ->
   GTot merkle_tree
 let mt_flush_to mt idx =
   let fhs = mt_flush_to_ 0 (MT?.hs mt) (MT?.i mt) idx (MT?.j mt) in
   MT idx (MT?.j mt) fhs (MT?.rhs_ok mt) (MT?.rhs mt) (MT?.mroot mt)
 
-val mt_flush: mt:wf_mt{MT?.j mt > MT?.i mt} -> GTot merkle_tree
+val mt_flush: mt:merkle_tree{mt_wf_elts mt /\ MT?.j mt > MT?.i mt} -> GTot merkle_tree
 let mt_flush mt = 
   mt_flush_to mt (MT?.j mt - 1)
 
